# imports: http://www.w3.org/2006/time#2016
# imports: https://ontology.unifiedcyberontology.org/uco/uco/1.4.0

@prefix drafting: <http://example.org/ontology/drafting/> .
@prefix owl: <http://www.w3.org/2002/07/owl#> .
@prefix rdf: <http://www.w3.org/1999/02/22-rdf-syntax-ns#> .
@prefix rdfs: <http://www.w3.org/2000/01/rdf-schema#> .
@prefix time: <http://www.w3.org/2006/time#> .
@prefix uco-action: <https://ontology.unifiedcyberontology.org/uco/action/> .
@prefix uco-core: <https://ontology.unifiedcyberontology.org/uco/core/> .
@prefix xsd: <http://www.w3.org/2001/XMLSchema#> .

<http://example.org/ontology/uco-time>
	a owl:Ontology ;
	owl:imports
		time:2016 ,
		<https://ontology.unifiedcyberontology.org/uco/uco/1.4.0>
		;
	.

drafting:Instant
	a owl:Class ;
	rdfs:subClassOf
		drafting:InstantaneousPerdurant ,
		time:Instant
		;
	.

drafting:InstantaneousPerdurant
	a owl:Class ;
	rdfs:subClassOf
		drafting:Perdurant ,
		[
			a owl:Restriction ;
			owl:onProperty time:hasTime ;
			owl:allValuesFrom time:Instant ;
		]
		;
	rdfs:isDefinedBy <https://github.com/ucoProject/UCO/issues/651> ;
	owl:disjointWith drafting:ProperIntervalicPerdurant ;
	.

drafting:IntervalicPerdurant
	a owl:Class ;
	rdfs:subClassOf
		drafting:Perdurant ,
		[
			a owl:Restriction ;
			owl:onProperty time:hasTime ;
			owl:allValuesFrom time:Interval ;
		]
		;
	rdfs:isDefinedBy <https://github.com/ucoProject/UCO/issues/651> ;
	.

drafting:Perdurant
	a owl:Class ;
	rdfs:subClassOf uco-core:UcoObject ;
	rdfs:isDefinedBy <https://github.com/ucoProject/UCO/issues/544> ;
	.

drafting:ProperIntervalicPerdurant
	a owl:Class ;
	rdfs:subClassOf
		drafting:IntervalicPerdurant ,
		[
			a owl:Restriction ;
			owl:onProperty time:hasTime ;
			owl:allValuesFrom time:ProperInterval ;
		]
		;
	rdfs:isDefinedBy <https://github.com/ucoProject/UCO/issues/651> ;
	owl:disjointWith drafting:InstantaneousPerdurant ;
	.

drafting:after
	a
		owl:ObjectProperty ,
		owl:IrreflexiveProperty ,
		owl:TransitiveProperty
		;
	rdfs:comment "The subject is a perdurant that occurs after the object. If a perdurant P1 is after another perdurant P2, then the beginning of P1 is after the end of P2.  (Definition adapted from OWL-Time's after.)"@en ;
	rdfs:domain drafting:Perdurant ;
	rdfs:isDefinedBy <https://github.com/ucoProject/UCO/issues/651> ;
	rdfs:range drafting:Perdurant ;
	rdfs:seeAlso time:after ;
	owl:inverseOf drafting:before ;
	.

drafting:before
	a
		owl:ObjectProperty ,
		owl:IrreflexiveProperty ,
		owl:TransitiveProperty
		;
	rdfs:comment "The subject is a perdurant that occurs before the object. If a perdurant P1 is before another perdurant P2, then the end of P1 is before the beginning of P2.  (Definition adapted from OWL-Time's before.)"@en ;
	rdfs:domain drafting:Perdurant ;
	rdfs:isDefinedBy <https://github.com/ucoProject/UCO/issues/651> ;
	rdfs:range drafting:Perdurant ;
	rdfs:seeAlso time:before ;
	owl:inverseOf drafting:after ;
	.

drafting:hasBeginning
	a owl:ObjectProperty ;
	rdfs:comment "Beginning of a perdurant.  (Definition adapted from OWL-Time's hasBeginning.)"@en ;
	rdfs:domain drafting:Perdurant ;
	rdfs:isDefinedBy <https://github.com/ucoProject/UCO/issues/651> ;
	rdfs:range drafting:InstantaneousPerdurant ;
	rdfs:seeAlso time:hasBeginning ;
	.

drafting:hasEnd
	a owl:ObjectProperty ;
	rdfs:comment "End of a perdurant.  (Definition adapted from OWL-Time's hasEnd.)"@en ;
	rdfs:domain drafting:Perdurant ;
	rdfs:isDefinedBy <https://github.com/ucoProject/UCO/issues/651> ;
	rdfs:range drafting:InstantaneousPerdurant ;
	rdfs:seeAlso time:hasEnd ;
	.

drafting:inside
	a owl:ObjectProperty ;
	rdfs:comment "An instantaneous perdurant that falls inside the intervalic perdurant. It is not intended to include beginnings and ends of intervalic perdurants.  (Definition adapted from OWL-Time's inside.)"@en ;
	rdfs:domain drafting:IntervalicPerdurant ;
	rdfs:isDefinedBy <https://github.com/ucoProject/UCO/issues/651> ;
	rdfs:range drafting:InstantaneousPerdurant ;
	.

drafting:intervalAfter
	a
		owl:ObjectProperty ,
		owl:IrreflexiveProperty
		;
	rdfs:subPropertyOf
		drafting:after ,
		drafting:intervalDisjoint
		;
	rdfs:comment "If a proper-intervalic perdurant P1 is intervalAfter another proper-intervalic perdurant P2, then the beginning of P1 is after the end of P2.  (Definition adapted from OWL-Time's intervalAfter.)"@en ;
	rdfs:domain drafting:ProperIntervalicPerdurant ;
	rdfs:isDefinedBy <https://github.com/ucoProject/UCO/issues/651> ;
	rdfs:range drafting:ProperIntervalicPerdurant ;
	rdfs:seeAlso time:intervalAfter ;
	owl:inverseOf drafting:intervalBefore ;
	.

drafting:intervalBefore
	a
		owl:ObjectProperty ,
		owl:IrreflexiveProperty
		;
	rdfs:subPropertyOf
		drafting:before ,
		drafting:intervalDisjoint
		;
	rdfs:comment "If a proper-intervalic perdurant P1 is intervalBefore another proper-intervalic perdurant P2, then the end of P1 is before the beginning of P2.  (Definition adapted from OWL-Time's intervalBefore.)"@en ;
	rdfs:domain drafting:ProperIntervalicPerdurant ;
	rdfs:isDefinedBy <https://github.com/ucoProject/UCO/issues/651> ;
	rdfs:range drafting:ProperIntervalicPerdurant ;
	rdfs:seeAlso time:intervalBefore ;
	owl:inverseOf drafting:intervalAfter ;
	.

drafting:intervalContains
	a owl:ObjectProperty ;
	rdfs:comment "If a proper-intervalic perdurant P1 is intervalContains another proper interval P2, then the beginning of P1 is before the beginning of P2, and the end of P1 is after the end of P2.  (Definition adapted from OWL-Time's intervalContains.)"@en ;
	rdfs:domain drafting:ProperIntervalicPerdurant ;
	rdfs:isDefinedBy <https://github.com/ucoProject/UCO/issues/651> ;
	rdfs:range drafting:ProperIntervalicPerdurant ;
	rdfs:seeAlso time:intervalContains ;
	owl:inverseOf drafting:intervalDuring ;
	.

drafting:intervalDisjoint
	a owl:ObjectProperty ;
	rdfs:comment "If a proper-intervalic perdurant P1 is intervalDisjoint another proper-intervalic perdurant P2, then the beginning of P1 is after the end of P2, or the end of P1 is before the beginning of P2, i.e. the perdurants' intervals do not overlap in any way, but their ordering relationship is not known.  (Definition adapted from OWL-Time's intervalDisjoint.)"@en ;
	rdfs:domain drafting:ProperIntervalicPerdurant ;
	rdfs:isDefinedBy <https://github.com/ucoProject/UCO/issues/651> ;
	rdfs:range drafting:ProperIntervalicPerdurant ;
	rdfs:seeAlso time:intervalDisjoint ;
	.

drafting:intervalDuring
	a owl:ObjectProperty ;
	rdfs:subPropertyOf drafting:intervalIn ;
	rdfs:comment "If a proper-intervalic perdurant P1 is intervalDuring another proper-intervalic perdurant P2, then the beginning of P1 is after the beginning of P2, and the end of P1 is before the end of P2.  (Definition adapted from OWL-Time's intervalDuring.)"@en ;
	rdfs:domain drafting:ProperIntervalicPerdurant ;
	rdfs:isDefinedBy <https://github.com/ucoProject/UCO/issues/651> ;
	rdfs:range drafting:ProperIntervalicPerdurant ;
	rdfs:seeAlso time:intervalDuring ;
	owl:inverseOf drafting:intervalContains ;
	.

drafting:intervalEquals
	a owl:ObjectProperty ;
	rdfs:comment "If a proper-intervalic perdurant P1 is intervalEquals another proper interval P2, then the beginning of P1 is coincident with the beginning of P2, and the end of P1 is coincident with the end of P2.  (Definition adapted from OWL-Time's intervalEquals.)"@en ;
	rdfs:domain drafting:ProperIntervalicPerdurant ;
	rdfs:isDefinedBy <https://github.com/ucoProject/UCO/issues/651> ;
	rdfs:range drafting:ProperIntervalicPerdurant ;
	rdfs:seeAlso time:intervalEquals ;
	owl:propertyDisjointWith drafting:intervalIn ;
	.

drafting:intervalFinishedBy
	a owl:ObjectProperty ;
	rdfs:comment "If a proper-intervalic perdurant P1 is intervalFinishedBy another proper-intervalic perdurant P2, then the beginning of P1 is before the beginning of P2, and the end of P1 is coincident with the end of P2.  (Definition adapted from OWL-Time's intervalFinishedBy.)"@en ;
	rdfs:domain drafting:ProperIntervalicPerdurant ;
	rdfs:isDefinedBy <https://github.com/ucoProject/UCO/issues/651> ;
	rdfs:range drafting:ProperIntervalicPerdurant ;
	rdfs:seeAlso time:intervalFinishedBy ;
	owl:inverseOf drafting:intervalFinishes ;
	.

drafting:intervalFinishes
	a owl:ObjectProperty ;
	rdfs:subPropertyOf drafting:intervalIn ;
	rdfs:comment "If a proper-intervalic perdurant P1 is intervalFinishes another proper-intervalic perdurant P2, then the beginning of P1 is after the beginning of P2, and the end of P1 is coincident with the end of P2.  (Definition adapted from OWL-Time's intervalFinishes.)"@en ;
	rdfs:domain drafting:ProperIntervalicPerdurant ;
	rdfs:isDefinedBy <https://github.com/ucoProject/UCO/issues/651> ;
	rdfs:range drafting:ProperIntervalicPerdurant ;
	rdfs:seeAlso time:intervalFinishes ;
	owl:inverseOf drafting:intervalFinishedBy ;
	.

drafting:intervalIn
	a owl:ObjectProperty ;
	rdfs:comment "If a proper-intervalic perdurant P1 is intervalIn another proper interval P2, then the beginning of P1 is after the beginning of P2 or is coincident with the beginning of P2, and the end of P1 is before the end of P2 or is coincident with the end of P2, except that end of P1 may not be coincident with the end of P2 if the beginning of P1 is coincident with the beginning of P2.  (Definition adapted from OWL-Time's intervalIn.)"@en ;
	rdfs:domain drafting:ProperIntervalicPerdurant ;
	rdfs:isDefinedBy <https://github.com/ucoProject/UCO/issues/651> ;
	rdfs:range drafting:ProperIntervalicPerdurant ;
	rdfs:seeAlso time:intervalIn ;
	owl:propertyDisjointWith drafting:intervalEquals ;
	.

drafting:intervalMeets
	a owl:ObjectProperty ;
	rdfs:comment "If a proper-intervalic perdurant P1 is intervalMeets another proper-intervalic perdurant P2, then the end of P1 is coincident with the beginning of P2.  (Definition adapted from OWL-Time's intervalMeets.)"@en ;
	rdfs:domain drafting:ProperIntervalicPerdurant ;
	rdfs:isDefinedBy <https://github.com/ucoProject/UCO/issues/651> ;
	rdfs:range drafting:ProperIntervalicPerdurant ;
	rdfs:seeAlso time:intervalMeets ;
	owl:inverseOf drafting:intervalMetBy ;
	.

drafting:intervalMetBy
	a owl:ObjectProperty ;
	rdfs:comment "If a proper-intervalic perdurant P1 is intervalMetBy another proper-intervalic perdurant P2, then the beginning of P1 is coincident with the end of P2.  (Definition adapted from OWL-Time's intervalMetBy.)"@en ;
	rdfs:domain drafting:ProperIntervalicPerdurant ;
	rdfs:isDefinedBy <https://github.com/ucoProject/UCO/issues/651> ;
	rdfs:range drafting:ProperIntervalicPerdurant ;
	rdfs:seeAlso time:intervalMetBy ;
	owl:inverseOf drafting:intervalMeets ;
	.

drafting:intervalOverlappedBy
	a owl:ObjectProperty ;
	rdfs:comment "If a proper-intervalic perdurant P1 is intervalOverlappedBy another proper-intervalic perdurant P2, then the beginning of P1 is after the beginning of P2, the beginning of P1 is before the end of P2, and the end of P1 is after the end of P2.  (Definition adapted from OWL-Time's intervalOverlappedBy.)"@en ;
	rdfs:domain drafting:ProperIntervalicPerdurant ;
	rdfs:isDefinedBy <https://github.com/ucoProject/UCO/issues/651> ;
	rdfs:range drafting:ProperIntervalicPerdurant ;
	rdfs:seeAlso time:intervalOverlappedBy ;
	owl:inverseOf drafting:intervalOverlaps ;
	.

drafting:intervalOverlaps
	a owl:ObjectProperty ;
	rdfs:comment "If a proper-intervalic perdurant P1 is intervalOverlaps another proper-intervalic perdurant P2, then the beginning of P1 is before the beginning of P2, the end of P1 is after the beginning of P2, and the end of P1 is before the end of P2.  (Definition adapted from OWL-Time's intervalOverlaps.)"@en ;
	rdfs:domain drafting:ProperIntervalicPerdurant ;
	rdfs:isDefinedBy <https://github.com/ucoProject/UCO/issues/651> ;
	rdfs:range drafting:ProperIntervalicPerdurant ;
	rdfs:seeAlso time:intervalOverlaps ;
	owl:inverseOf drafting:intervalOverlappedBy ;
	.

drafting:intervalStartedBy
	a owl:ObjectProperty ;
	rdfs:comment "If a proper-intervalic perdurant P1 is intervalStarted another proper-intervalic perdurant P2, then the beginning of P1 is coincident with the beginning of P2, and the end of P1 is after the end of P2.  (Definition adapted from OWL-Time's intervalStartedBy.)"@en ;
	rdfs:domain drafting:ProperIntervalicPerdurant ;
	rdfs:isDefinedBy <https://github.com/ucoProject/UCO/issues/651> ;
	rdfs:range drafting:ProperIntervalicPerdurant ;
	rdfs:seeAlso time:intervalStartedBy ;
	owl:inverseOf drafting:intervalStarts ;
	.

drafting:intervalStarts
	a owl:ObjectProperty ;
	rdfs:subPropertyOf drafting:intervalIn ;
	rdfs:comment "If a proper-intervalic perdurant P1 is intervalStarts another proper-intervalic perdurant P2, then the beginning of P1 is coincident with the beginning of P2, and the end of P1 is before the end of P2.  (Definition adapted from OWL-Time's intervalStarts.)"@en ;
	rdfs:domain drafting:ProperIntervalicPerdurant ;
	rdfs:isDefinedBy <https://github.com/ucoProject/UCO/issues/651> ;
	rdfs:range drafting:ProperIntervalicPerdurant ;
	rdfs:seeAlso time:intervalStarts ;
	owl:inverseOf drafting:intervalStartedBy ;
	.

uco-action:Action
	rdfs:subClassOf drafting:Perdurant ;
	.

uco-action:subaction
	rdfs:subPropertyOf drafting:intervalDuring ;
	.

uco-core:Event
	rdfs:subClassOf drafting:Perdurant ;
	.

[]
	a owl:Axiom ;
	rdfs:isDefinedBy <https://github.com/ucoProject/UCO/issues/544> ;
	owl:annotatedProperty rdfs:subClassOf ;
	owl:annotatedSource uco-action:Action ;
	owl:annotatedTarget drafting:Perdurant ;
	.

[]
	a owl:Axiom ;
	rdfs:isDefinedBy <https://github.com/ucoProject/UCO/issues/544> ;
	owl:annotatedProperty rdfs:subClassOf ;
	owl:annotatedSource uco-core:Event ;
	owl:annotatedTarget drafting:Perdurant ;
	.

[]
	a owl:Axiom ;
	rdfs:isDefinedBy <https://github.com/ucoProject/UCO/issues/651> ;
	owl:annotatedProperty rdfs:subPropertyOf ;
	owl:annotatedSource uco-action:subaction ;
	owl:annotatedTarget drafting:intervalDuring ;
	.

